Rename RPCClient_own to is_RPCClient

src/program_proof/fencing/config_proof.v
@@ -3,6 +3,7 @@ From Goose.github_com.mit_pdos.gokv.fencing Require Import frontend.
 From Perennial.program_proof Require Import grove_prelude.
 From Perennial.program_proof.memkv Require Export urpc_lib urpc_proof urpc_spec.
 From Perennial.program_proof.fencing Require Export ctr_proof.
+From Perennial.program_proof Require Export marshal_proof.
 From iris.base_logic Require Import mono_nat.
 
 Module config.
@@ -11,23 +12,51 @@ Context `{!heapGS Σ}.
 
 Record names :=
   {
-
+    urpc_gn:server_chan_gnames
   }.
 
 Context (γ:names).
 
-Definition is_host (host:u64) (epoch_tok : u64 → iProp Σ) (host_inv:u64 → iProp Σ): iProp Σ.
-Admitted.
+Program Definition Get_spec host_inv :=
+  λ (reqData:list u8), λne (Φ : list u8 -d> iPropO Σ),
+  (∀ v l, ⌜has_encoding l [EncUInt64 v]⌝ -∗ host_inv v -∗ Φ l)%I
+.
+Next Obligation.
+  solve_proper.
+Defined.
 
-Global Instance is_host_pers host epoch_tok host_inv : Persistent (is_host host epoch_tok host_inv).
-Admitted.
+Program Definition AcquireEpoch_spec epoch_tok host_inv :=
+  λ (reqData:list u8), λne (Φ : list u8 -d> iPropO Σ),
+  (∃ newhost, ⌜has_encoding reqData [EncUInt64 newhost]⌝ ∗
+  host_inv newhost ∗
+  (∀ l epoch, ⌜has_encoding l [EncUInt64 epoch]⌝ -∗ epoch_tok epoch -∗ Φ l))%I
+.
+Next Obligation.
+  solve_proper.
+Defined.
 
-Definition is_Clerk (ck:loc) : iProp Σ.
-Admitted.
+Program Definition trivial_spec :=
+  λ (reqData:list u8), λne (Φ : list u8 -d> iPropO Σ),
+  (∀ (l:list u8), True -∗ Φ l)%I
+.
+Next Obligation.
+  solve_proper.
+Defined.
 
-Global Instance is_Clerk_pers ck : Persistent (is_Clerk ck).
-Admitted.
+Context `{!rpcregG Σ}.
 
+Definition is_host (host:u64) (epoch_tok : u64 → iProp Σ) (host_inv:u64 → iProp Σ): iProp Σ :=
+  handler_spec γ.(urpc_gn) host (U64 0) (AcquireEpoch_spec epoch_tok host_inv) ∗
+  handler_spec γ.(urpc_gn) host (U64 1) (Get_spec host_inv) ∗
+  handler_spec γ.(urpc_gn) host (U64 2) trivial_spec ∗
+  handlers_dom γ.(urpc_gn) {[ (U64 0) ; (U64 1) ; (U64 2)]}
+.
+
+Definition is_Clerk (ck:loc) (host:u64): iProp Σ :=
+  ∃ (cl:loc),
+    "#Hcl" ∷ readonly (ck ↦[Clerk :: "cl"] #cl) ∗
+    "#His_cl" ∷ is_RPCClient cl host
+.
 
 Lemma wp_MakeClerk host epoch_tok host_inv :
   is_host host epoch_tok host_inv -∗
@@ -36,14 +65,30 @@ Lemma wp_MakeClerk host epoch_tok host_inv :
   }}}
     config.MakeClerk #host
   {{{
-        (ck:loc), RET #ck; is_Clerk ck
+        (ck:loc), RET #ck; is_Clerk ck host
   }}}.
 Proof.
-Admitted.
+  iIntros "#Hhost !#" (Φ) "_ HΦ".
+  wp_lam.
+  wp_apply (wp_allocStruct).
+  { naive_solver. }
+  iIntros (ck) "Hck".
+  wp_pures.
+  iDestruct (struct_fields_split with "Hck") as "HH".
+  iNamed "HH".
+  wp_apply (wp_MakeClient).
+  iIntros (?) "#His_cl".
+  wp_storeField.
+  iMod (readonly_alloc_1 with "cl") as "#Hcl".
+  iApply "HΦ".
+  iModIntro.
+  iExists _.
+  iFrame "#".
+Qed.
 
 Lemma wp_Clerk__AcquireEpoch ck host newHost epoch_tok host_inv :
   is_host host epoch_tok host_inv -∗
-  is_Clerk ck -∗
+  is_Clerk ck host -∗
   {{{
         True
   }}}
@@ -56,7 +101,7 @@ Admitted.
 
 Lemma wp_Clerk__Get ck host epoch_tok host_inv :
   is_host host epoch_tok host_inv -∗
-  is_Clerk ck -∗
+  is_Clerk ck host -∗
   {{{
         True
   }}}
